src/ReactorModel/Objects/Reactor/Finite.lean
@@ -1,13 +1,13 @@
-import ReactorModel.Objects.Reactor.Indexable
+import ReactorModel.Objects.Reactor.Hierarchical
 
 noncomputable section
 
 namespace Reactor
 
-class Finite (α) [Indexable α] where
+class Finite (α) [Hierarchical α] where
   fin : ∀ (rtr : α) (cpt : Component), rtr[cpt].Finite
 
-def Finite.ids [Indexable α] [Finite α] (rtr : α) (cpt : Component) : List cpt.idType :=
+def Finite.ids [Hierarchical α] [Finite α] (rtr : α) (cpt : Component) : List cpt.idType :=
   (fin rtr cpt).toFinset.toList 
 
 namespace Reactor
