src/ReactorModel/Objects/Reactor.lean
@@ -1,7 +1,7 @@
 import ReactorModel.Objects.Reactor.Basic
 import ReactorModel.Objects.Reactor.Extensional
 import ReactorModel.Objects.Reactor.Finite
-import ReactorModel.Objects.Reactor.Indexable
+import ReactorModel.Objects.Reactor.Hierarchical
 import ReactorModel.Objects.Reactor.Proper
 import ReactorModel.Objects.Reactor.Theorems
 import ReactorModel.Objects.Reactor.Updatable
