src/ReactorModel/Objects/Reactor/Theorems.lean
@@ -2,6 +2,6 @@ import ReactorModel.Objects.Reactor.Theorems.Accessible
 import ReactorModel.Objects.Reactor.Theorems.Basic
 import ReactorModel.Objects.Reactor.Theorems.Extensional
 import ReactorModel.Objects.Reactor.Theorems.Finite
-import ReactorModel.Objects.Reactor.Theorems.Indexable
+import ReactorModel.Objects.Reactor.Theorems.Hierarchical
 import ReactorModel.Objects.Reactor.Theorems.Proper
 import ReactorModel.Objects.Reactor.Theorems.Readable
