src/ReactorModel/Objects/Reactor/Theorems/Finite.lean
@@ -1,5 +1,5 @@
 import ReactorModel.Objects.Reactor.Finite
 
-theorem Reactor.mem_ids_iff [Indexable α] [Finite α] {rtr : α} {i} : 
+theorem Reactor.mem_ids_iff [Hierarchical α] [Finite α] {rtr : α} {i} : 
     (i ∈ Finite.ids rtr cpt) ↔ (∃ o, rtr[cpt][i] = some o) := by
   simp [Finite.ids, ←Partial.mem_def, Partial.mem_iff]
